

UNIVERSITY NAME

DOCTORAL THESIS

---

# Thesis Title

---

*Author:*  
John SMITH

*Supervisor:*  
Dr. James SMITH

*A thesis submitted in fulfillment of the requirements  
for the degree of Doctor of Philosophy  
in the*

Research Group Name  
Department or School Name

April 26, 2021

*“Thanks to my solid academic training, today I can write hundreds of words on virtually any topic without possessing a shred of information, which is how I got a good job in journalism.”*

Dave Barry

UNIVERSITY NAME

# *Abstract*

Faculty Name  
Department or School Name

Doctor of Philosophy

**Thesis Title**

by John SMITH

The Thesis Abstract is written here (and usually kept to just this page). The page is kept centered vertically so can expand into the blank space above the title too...



## *Acknowledgements*

The acknowledgments and the people to thank go here, don't forget to include your project advisor. . .



# Contents

<b>Abstract</b>	<b>iii</b>
<b>Acknowledgements</b>	<b>v</b>
<b>1 Proving semantic preservation in HILECOP</b>	<b>1</b>
1.1 Preliminary Definitions . . . . .	1
1.2 Behavior Preservation Theorem . . . . .	1
1.2.1 Proof Notations . . . . .	1
1.2.2 Behavior Preservation Theorem and Proof . . . . .	1
1.2.3 Bisimulation Theorem and Proof . . . . .	3
1.3 Initial States . . . . .	6
1.4 First Rising Edge . . . . .	6
1.5 Rising Edge . . . . .	6
1.6 Falling Edge . . . . .	6
1.6.1 Falling Edge and marking . . . . .	8
1.6.2 Falling edge and time counters . . . . .	14
1.6.3 Falling edge and firable transitions . . . . .	19
1.7 A detailed proof: equivalence of fired transitions . . . . .	19
<b>A Reminder on natural semantics</b>	<b>21</b>
<b>B Reminder on induction principles</b>	<b>23</b>





# List of Figures



# List of Tables



*For/Dedicated to/To my...*



## Chapter 1

# Proving semantic preservation in HILECOP

- Change  $\sigma_{injr}$  and  $\sigma_{injf}$  into  $\sigma_i$ .
- Define the  $\text{Inject}_\downarrow$  and  $\text{Inject}_\uparrow$  relations.
- Keep the  $sitpn$  argument in the SITPN full execution relation, but remove it from the SITPN execution, cycle and state transition relations.

### 1.1 Preliminary Definitions

### 1.2 Behavior Preservation Theorem

#### 1.2.1 Proof Notations

- Frame box for pending goals:  $\boxed{\forall n \in \mathbb{N}, n > 0 \vee n = 0}$
- Red frame box for completed goals:  $\boxed{\text{true} = \text{true}}$
- Green frame box for induction hypotheses:

$$\boxed{\forall n \in \mathbb{N}, n + 1 > 0}$$

- **CASE** to denote a case during a proof by case analysis.

Make a list of all signals and constants of the T and P components, and their related aliases.

#### 1.2.2 Behavior Preservation Theorem and Proof

**Theorem 1** (Behavior Preservation). *For all  $sitpn \in \text{SITPN}$ ,  $d \in \text{design}$ ,  $\gamma \in \text{WM}(sitpn, d)$ ,  $\tau \in \mathbb{N}$ ,  $E_c \in \mathbb{N} \rightarrow \mathcal{C} \rightarrow \mathbb{B}$ ,  $\theta_s \in \text{list}(S(sitpn))$  s.t.*

- *SITPN  $sitpn$  translates into design  $d$ :  $\lfloor sitpn \rfloor_{\mathcal{H}} = (d, \gamma)$*
- *SITPN  $sitpn$  yields the execution trace  $\theta_s$  after  $\tau$  execution cycles in environment  $E_c$ :*  

$$E_c, \tau \vdash sitpn \xrightarrow{\text{full}} \theta_s.$$

Constants and signals reference			
Full name	Alias	Category	Type
"input_conditions"	"ic"	input port (T)	$\mathbb{B}$
"input_conditions"	"ic"	input port (T)	$\mathbb{B}$
"reinit_time"	"rt"	input port (T)	$\mathbb{B}$
"input_arcs_valid"	"iav"	input port (T)	$\mathbb{B}$
"fired"	"f"	output port (T)	$\mathbb{B}$
"s_condition_combination"	"scc"	internal signal (T)	$\mathbb{B}$
"s_reinit_time_counter"	"srtc"	internal signal (T)	$\mathbb{B}$
"s_priority_combination"	"spc"	internal signal (T)	$\mathbb{B}$
"s_fired"	"sf"	internal signal (T)	$\mathbb{B}$
"s_firable"	"sfa"	internal signal (T)	$\mathbb{B}$
"s_enabled"	"se"	internal signal (T)	$\mathbb{B}$
"input_arcs_number"	"ian"	generic constant (T)	$\mathbb{N}$
"transition_type"	"tt"	generic constant (T)	$\{\text{NOT\_TEMP, TEMP\_A\_B, TEMP\_A\_A, TEMP\_A\_INF}\}$
"conditions_number"	"cn"	generic constant (T)	$\mathbb{N}$
"maximal_time_counter"	"mtc"	generic constant (T)	$\mathbb{N}$
"s_marking"	"sm"	internal signal (P)	$\mathbb{N}$
"s_output_token_sum"	"sots"	internal signal (P)	$\mathbb{N}$
"s_input_token_sum"	"sits"	internal signal (P)	$\mathbb{N}$
"reinit_transition_time"	"rtt"	output port (P)	$\mathbb{B}$
"output_arcs_types"	"oat"	input port (P)	$\{\text{BASIC, TEST, INHIB}\}$
"output_arcs_weights"	"oaw"	input port (P)	$\mathbb{N}$
"output_transition_fired"	"otf"	input port (P)	$\mathbb{B}$
"input_arcs_weights"	"iaw"	input port (P)	$\mathbb{N}$
"input_transition_fired"	"itf"	input port (P)	$\mathbb{B}$

then there exists  $\Delta \in \text{ElDesign}(d, \mathcal{D}_{\mathcal{H}})$  s.t. for all  $E_p \in (\mathbb{N} \times \{\uparrow, \downarrow\}) \rightarrow \text{Ins}(\Delta) \rightarrow \text{value}$  verifying

- Simulation/Execution environments are similar:  $\gamma \vdash E_p \stackrel{\text{env}}{=} E_c$ .

then there exists  $\theta_\sigma \in \text{list}(\Sigma(\Delta))$  s.t.

- Under the HILECOP design store  $\mathcal{D}_{\mathcal{H}}$  and with an empty generic constant dimensioning function, design  $d$  yields the simulation trace  $\theta_\sigma$  after  $\tau$  simulation cycles, starting from its initial state:

$$\mathcal{D}_{\mathcal{H}}, \Delta, \emptyset, E_p, \tau \vdash d \xrightarrow{\text{full}} \theta_\sigma$$

- Traces  $\theta_s$  and  $\theta_\sigma$  are similar:  $\theta_s \sim \theta_\sigma$

*Proof.*  $\boxed{\exists \Delta, \forall E_p, \gamma \vdash E_p \stackrel{\text{env}}{=} E_c, \exists \theta_\sigma, \mathcal{D}_{\mathcal{H}}, \Delta, \emptyset, E_p, \tau \vdash d \xrightarrow{\text{full}} \theta_\sigma \wedge \theta_s \sim \theta_\sigma}$

By definition of the  $\mathcal{H}$ -VHDL full simulation relation:

$\mathcal{D}_{\mathcal{H}}, \Delta, \emptyset, E_p, \tau \vdash d \xrightarrow{\text{full}} \theta_\sigma \equiv \exists \sigma_e, \sigma_0 \in \Sigma(\Delta), \mathcal{D}_{\mathcal{H}}, \emptyset \vdash d \xrightarrow{\text{elab}} (\Delta, \sigma_e)$  and  $\mathcal{D}_{\mathcal{H}}, \Delta, \sigma_e \vdash d.cs \xrightarrow{\text{init}} \sigma_0$  and  $\mathcal{D}_{\mathcal{H}}, E_p, \Delta, \tau, \sigma_0 \vdash d.cs \rightarrow \theta_\sigma$ .



Use **Elaboration**, **Initialization** and **Simulation** theorems to show that there exists a  $\Delta, \theta_\sigma, \sigma_e$  and  $\sigma_0$  such that  $\mathcal{D}_H, \emptyset \vdash d \xrightarrow{elab} (\Delta, \sigma_e)$  and  $\mathcal{D}_H, \Delta, \sigma_e \vdash d.cs \xrightarrow{init} \sigma_0$  and  $\mathcal{D}_H, E_p, \Delta, \tau, \sigma_0 \vdash d.cs \rightarrow \theta_\sigma$ .

Use **Full Bisimulation** theorem to show traces similarity.

□

**Theorem 2** (Elaboration). *For all  $sitpn \in SITPN, d \in design, \gamma \in WM(sitpn, d)$  s.t.*

- $\lfloor sitpn \rfloor_H = (d, \gamma)$

*then there exists  $\Delta \in ElDesign(d, \mathcal{D}_H), \sigma_e \in \Sigma(\Delta)$  s.t.*

- $\mathcal{D}_H, \emptyset \vdash d \xrightarrow{elab} (\Delta, \sigma_e)$

**Theorem 3** (Initialization). *For all  $sitpn \in SITPN, d \in design, \gamma \in WM(sitpn, d), \Delta \in ElDesign(d, \mathcal{D}_H), \sigma_e \in \Sigma(\Delta)$  s.t.*

- $\lfloor sitpn \rfloor_H = (d, \gamma)$  and  $\mathcal{D}_H, \emptyset \vdash d \xrightarrow{elab} (\Delta, \sigma_e)$

*then there exists  $\sigma_0 \in \Sigma(\Delta)$  s.t.*

- $\sigma_0$  is the initial simulation state:  $\mathcal{D}_H, \Delta, \sigma_e \vdash d.cs \xrightarrow{init} \sigma_0$

**Theorem 4** (Simulation). *For all  $sitpn \in SITPN, d \in design, \gamma \in WM(sitpn, d), \Delta \in ElDesign(d, \mathcal{D}_H), \sigma_e, \sigma_0 \in \Sigma(\Delta)$  s.t.*

- $\lfloor sitpn \rfloor_H = (d, \gamma)$  and  $\mathcal{D}_H, \emptyset \vdash d \xrightarrow{elab} (\Delta, \sigma_e)$  and  $\mathcal{D}_H, \Delta, \sigma_e \vdash d.cs \xrightarrow{init} \sigma_0$

*then for all  $E_p \in (\mathbb{N} \times \{\uparrow, \downarrow\}) \rightarrow Ins(\Delta) \rightarrow value, \tau \in \mathbb{N}$ , there exists  $\theta_\sigma \in list(\Sigma(\Delta))$  s.t.*

- *Design  $d$  yields the simulation trace  $\theta_\sigma$  after  $\tau$  simulation cycles, starting from initial state  $\sigma_0$ :*  
 $\mathcal{D}_H, E_p, \Delta, \tau, \sigma_0 \vdash d.cs \rightarrow \theta_\sigma$

### 1.2.3 Bisimulation Theorem and Proof

**Theorem 5** (Full Bisimulation). *For all  $sitpn \in SITPN, d \in design, \gamma \in WM(sitpn, d), \tau \in \mathbb{N}, E_c \in \mathbb{N} \rightarrow \mathcal{C} \rightarrow \mathbb{B}, \theta_s \in list(S(sitpn)), \Delta \in ElDesign(d, \mathcal{D}_H), E_p \in (\mathbb{N} \times \{\uparrow, \downarrow\}) \rightarrow Ins(\Delta) \rightarrow value, \theta_\sigma \in list(\Sigma(\Delta))$  s.t.*

- $\lfloor sitpn \rfloor_H = (d, \gamma)$
- $\gamma \vdash E_p \stackrel{env}{=} E_c$
- $E_c, \tau \vdash sitpn \xrightarrow{full} \theta_s$
- $\mathcal{D}_H, \Delta, \emptyset, E_p, \tau \vdash d \xrightarrow{full} \theta_\sigma$

*then  $\theta_s \sim \theta_\sigma$*

*Proof.* Case analysis on  $\tau$  (2 CASES).

- **CASE**  $\tau = 0$ . By definition of the SITPN full execution and the  $\mathcal{H}$ -VHDL full simulation relations:

- $\mathcal{D}_{\mathcal{H}}, \emptyset \vdash d \xrightarrow{elab} (\Delta, \sigma_e)$
- $\Delta, \sigma_e \vdash d.cs \xrightarrow{init} \sigma_0$
- $\theta_s = [s_0]$  and  $\theta_\sigma = [\sigma_0]$

$\boxed{\gamma \vdash s_0 \sim \sigma_0}$  (by def. of similar execution trace relation). Solved by applying Lemma ??.

- **CASE**  $\tau > 0$ . By definition of the SITPN full execution and the  $\mathcal{H}$ -VHDL full execution relations:

- $E_c, \tau \vdash s_0 \xrightarrow{\uparrow_0} s_0$
- $E_c, \tau \vdash s_0 \xrightarrow{\downarrow} s$
- $E_c, \tau - 1 \vdash sitpn, s \rightarrow \theta_s$
- $\mathcal{D}_{\mathcal{H}}, \emptyset \vdash d \xrightarrow{elab} (\Delta, \sigma_e)$
- $\Delta, \sigma_e \vdash d.cs \xrightarrow{init} \sigma_0$
- $E_p, \Delta, \tau, \sigma_0 \vdash d.cs \rightarrow \theta$

$\boxed{\gamma \vdash (s_0 :: s :: \theta_s) \sim (\sigma_0 :: \theta)}$

By definition of the  $\mathcal{H}$ -VHDL full simulation relation, we know:

- $E_p, \Delta, \tau, \sigma_0 \vdash d.cs \xrightarrow{\uparrow, \downarrow} \sigma$
- $E_p, \Delta, \tau - 1, \sigma \vdash d.cs \rightarrow \theta_\sigma$

where  $\theta = \sigma :: \theta_\sigma$ .

Rewriting  $\theta$  as  $\sigma :: \theta_\sigma$ ,  $\boxed{\gamma \vdash (s_0 :: s :: \theta_s) \sim (\sigma_0 :: \sigma :: \theta_\sigma)}$

3 subgoals (by def. of ??).

1.  $\gamma \vdash s_0 \sim \sigma_0$  (solved by applying Lemma ??).
2.  $\gamma \vdash s \sim \sigma$  (solved by applying Lemma **First Cycle**).
3.  $\gamma \vdash \theta_s \sim \theta_\sigma$  (solved by applying Lemma **Bisimulation**).

□

**Lemma 1** (First Cycle). *For all  $sitpn \in SITPN, d \in design, \gamma \in WM(sitpn, d), s \in S(sitpn), \Delta \in ElDesign(d, \mathcal{D}_{\mathcal{H}}), \sigma_e, \sigma_0, \sigma \in \Sigma(\Delta), E_c \in \mathbb{N} \rightarrow \mathcal{C} \rightarrow \mathbb{B}, E_p \in (\mathbb{N} \times \{\uparrow, \downarrow\}) \rightarrow Ins(\Delta) \rightarrow value$ , assume that:*

- $[sitpn]_{\mathcal{H}} = (d, \gamma)$  and  $\mathcal{D}_{\mathcal{H}}, \emptyset \vdash d \xrightarrow{elab} (\Delta, \sigma_e)$  and  $\gamma \vdash E_p \stackrel{env}{=} E_c$
- $\sigma_0$  is the initial state of  $\Delta$ :  $\Delta, \sigma_e \vdash d.cs \xrightarrow{init} \sigma_0$

- First execution cycle for  $d$ :  $E_p, \Delta, \tau, \sigma_0 \vdash d.cs \xrightarrow{\uparrow, \downarrow} \sigma$
- Particular first execution cycle for  $sitpn$  (first rising edge is idle):  
 $E_c, \tau \vdash s_0 \xrightarrow{\uparrow_0} s_0$  and  $E_c, \tau \vdash s_0 \xrightarrow{\downarrow} s$

then  $\gamma \vdash s \xrightarrow{\downarrow} \sigma$ .

*Proof.* Let's show that the first execution cycle leads to two states verifying the ?? relation:  $\gamma \vdash s \xrightarrow{\downarrow} \sigma$ .

By definition of the  $\mathcal{H}$ -VHDL cycle relation, we have:

- $\text{Inject}_{\uparrow}(\sigma_0, E_p, \tau, \sigma_{injr})$  and  $\Delta, \sigma_{injr} \vdash d.cs \xrightarrow{\uparrow} \sigma_r$  and  $\Delta, \sigma_r \vdash d.cs \xrightarrow{\theta} \sigma'$
- $\text{Inject}_{\downarrow}(\sigma', E_p, \tau, \sigma_{injf})$  and  $\Delta, \sigma_{injf} \vdash d.cs \xrightarrow{\downarrow} \sigma_f$  and  $\Delta, \sigma_f \vdash d.cs \xrightarrow{\theta'} \sigma$

Then, we can apply the **Falling Edge** lemma to solve  $\gamma \vdash s \xrightarrow{\downarrow} \sigma$ .

One premise of the **Falling Edge** lemma remains to be proved:  $\gamma, E_c, \tau \vdash s_0 \xrightarrow{\uparrow} \sigma'$ .

Then, we can apply the ?? lemma to solve  $\gamma, E_c, \tau \vdash s_0 \xrightarrow{\uparrow} \sigma'$ .

□

**Lemma 2** (Bisimulation). *For all  $sitpn, d, \gamma, E_p, E_c, \tau, s, \theta_s, \sigma, \theta_\sigma, \Delta, \sigma_e$ , assume that:*

- $[sitpn]_{\mathcal{H}} = (d, \gamma)$  and  $\gamma \vdash E_p \stackrel{env}{=} E_c$  and  $\mathcal{D}_{\mathcal{H}}, \emptyset \vdash d \xrightarrow{elab} \Delta, \sigma_e$
- Starting states are similar as intended after a falling edge:  $\gamma \vdash s \xrightarrow{\downarrow} \sigma$
- $E_c, \tau \vdash sitpn, s \rightarrow \theta_s$
- $E_p, \Delta, \tau, \sigma \vdash d.cs \rightarrow \theta_\sigma$

then  $\gamma \vdash \theta_s \sim \theta_\sigma$ .

*Proof.* Induction on  $\tau$ .

- Base case,  $\tau = 0$ : traces are empty, trivial.
- Induction case,  $\tau > 0$ :

$\forall s, \sigma, \theta_s, \theta_\sigma$  s.t.  $\gamma \vdash s \xrightarrow{\downarrow} \sigma$  and  $E_c, \tau - 1 \vdash sitpn, s \rightarrow \theta_s$  and  $E_p, \Delta, \tau - 1, \sigma \vdash d.cs \rightarrow \theta_\sigma$   
then  $\gamma \vdash \theta_s \sim \theta_\sigma$ .

By definition of the SITPN execution and the  $\mathcal{H}$ -VHDL simulation relations for  $\tau > 0$ :

- $E, \tau \vdash sitpn, s \xrightarrow{\uparrow, \downarrow} s'$  and  $E_c, \tau - 1 \vdash sitpn, s \rightarrow \theta_s$ .
- $E_p, \Delta, \tau, \sigma \vdash d.cs \xrightarrow{\uparrow, \downarrow} \sigma'$  and  $E_p, \Delta, \tau - 1, \sigma \vdash d.cs \rightarrow \theta_\sigma$ .

$$\boxed{\gamma \vdash (s' :: \theta_s) \sim (\sigma' :: \theta_\sigma)}.$$

2 subgoals (by def. of ??).

1.  $\boxed{\gamma \vdash s' \sim \sigma'}$  (solved with **Step**).
2.  $\boxed{\gamma \vdash \theta_s \sim \theta_\sigma}$  (solved with **Step** and IH).

□

**Lemma 3 (Step).** *For all sitpn,  $d, \gamma, E_p, E_c, \tau, s, s'', \sigma, \sigma'', \Delta, \sigma_e$ , assume that:*

- $\llbracket \text{sitpn} \rrbracket_{\mathcal{H}} = (d, \gamma)$  and  $E_p \stackrel{env}{=} E_c$  and  $\mathcal{D}_{\mathcal{H}}, \emptyset \vdash d \xrightarrow{elab} \Delta, \sigma_e$
- $\gamma \vdash s \stackrel{\downarrow}{\sim} \sigma$
- From state  $s$  to  $s''$  in one execution cycle:  $E_c, \tau \vdash \text{sitpn}, s \xrightarrow{\uparrow, \downarrow} s''$
- From state  $\sigma$  to  $\sigma''$  in one simulation cycle:  $E_p, \Delta, \tau, \sigma \vdash d.cs \xrightarrow{\uparrow, \downarrow} \sigma''$

then  $\gamma \vdash s'' \stackrel{\downarrow}{\sim} \sigma''$ .

*Proof.* By def. of the SITPN and  $\mathcal{H}$ -VHDL cycle relations:

- $E_c, \tau \vdash \text{sitpn}, s \xrightarrow{\uparrow} s'$  and  $E_c, \tau \vdash \text{sitpn}, s' \xrightarrow{\downarrow} s''$
- $\text{Inject}_{\uparrow}(\sigma, E_p, \tau, \sigma_{injr})$  and  $\Delta, \sigma_{injr} \vdash d.cs \xrightarrow{\uparrow} \sigma_r$  and  $\Delta, \sigma_r \vdash d.cs \xrightarrow{\theta} \sigma'$
- $\text{Inject}_{\downarrow}(\sigma', E_p, \tau, \sigma_{injf})$  and  $\Delta, \sigma_{injf} \vdash d.cs \xrightarrow{\downarrow} \sigma_f$  and  $\Delta, \sigma_f \vdash d.cs \xrightarrow{\theta'} \sigma''$

Solved by applying ?? and then “Falling Edge” lemmas.

□

### 1.3 Initial States

### 1.4 First Rising Edge

### 1.5 Rising Edge

### 1.6 Falling Edge

**Definition 1 (Falling Edge Hypotheses).** *Given an sitpn  $\in \text{SITPN}$ ,  $d \in \text{design}$ ,  $\gamma \in \text{WM}(\text{sitpn}, d)$ ,  $E_c \in \mathbb{N} \rightarrow \mathcal{C} \rightarrow \mathbb{B}$ ,  $\Delta \in \text{ElDesign}(d, \mathcal{D}_{\mathcal{H}})$ ,  $E_p \in (\mathbb{N} \times \{\uparrow, \downarrow\}) \rightarrow \text{Ins}(\Delta) \rightarrow \text{value}$ ,  $\tau \in \mathbb{N}$ ,  $s, s' \in S(\text{sitpn})$ ,  $\sigma_e, \sigma, \sigma_i, \sigma_{\downarrow}, \sigma' \in \Sigma(\Delta)$ , assume that:*

- $\llbracket \text{sitpn} \rrbracket_{\mathcal{H}} = (d, \gamma)$  and  $\gamma \vdash E_p \stackrel{env}{=} E_c$  and  $\mathcal{D}_{\mathcal{H}}, \emptyset \vdash d \xrightarrow{elab} \Delta, \sigma_e$
- $\gamma, E_c, \tau \vdash s \stackrel{\uparrow}{\sim} \sigma$

- $E_c, \tau \vdash s \xrightarrow{\downarrow} s'$
- $\text{Inject}_{\downarrow}(\sigma, E_p, \tau, \sigma_i)$  and  $\Delta, \sigma_i \vdash \text{d.cs} \xrightarrow{\downarrow} \sigma_{\downarrow}$  and  $\Delta, \sigma_{\downarrow} \vdash \text{d.cs} \xrightarrow{\sim} \sigma'$
- State  $\sigma$  is a stable design state:  $\mathcal{D}_{\mathcal{H}}, \Delta, \sigma \vdash \text{d.cs} \xrightarrow{\text{comb}} \sigma$

**Lemma 4** (Falling Edge). For all sitpn,  $d, \gamma, \Delta, \sigma_e, E_c, E_p, \tau, s, s', \sigma, \sigma_i, \sigma_{\downarrow}, \sigma'$  that verify the hypotheses of Def. 1, then  $\gamma \vdash s' \xrightarrow{\downarrow} \sigma'$ .

*Proof.* By definition of ??, there are 12 points to prove.

1.  $\forall p \in P, id_p \in \text{Comps}(\Delta) \text{ s.t. } \gamma(p) = id_p, s'.M(p) = \sigma'(id_p)("s\_marking").$
2.  $\forall t \in T_i, id_t \in \text{Comps}(\Delta) \text{ s.t. } \gamma(t) = id_t,$   
 $(upper(I_s(t)) = \infty \wedge s'.I(t) \leq lower(I_s(t)) \Rightarrow s'.I(t) = \sigma'(id_t)("s\_time\_counter"))$   
 $\wedge (upper(I_s(t)) = \infty \wedge s'.I(t) > lower(I_s(t)) \Rightarrow \sigma'(id_t)("s\_time\_counter") = lower(I_s(t)))$   
 $\wedge (upper(I_s(t)) \neq \infty \wedge s'.I(t) > upper(I_s(t)) \Rightarrow \sigma'(id_t)("s\_time\_counter") = upper(I_s(t)))$   
 $\wedge (upper(I_s(t)) \neq \infty \wedge s'.I(t) \leq upper(I_s(t)) \Rightarrow s'.I(t) = \sigma'(id_t)("s\_time\_counter")).$
3.  $\forall t \in T_i, id_t \in \text{Comps}(\Delta) \text{ s.t. } \gamma(t) = id_t, s'.reset_t(t) = \sigma'(id_t)("s\_reinit\_time\_counter").$
4.  $\forall c \in C, id_c \in \text{Ins}(\Delta) \text{ s.t. } \gamma(c) = id_c, s'.cond(c) = \sigma'(id_c).$
5.  $\forall a \in \mathcal{A}, id_a \in \text{Outs}(\Delta) \text{ s.t. } \gamma(a) = id_a, s'.ex(a) = \sigma'(id_a).$
6.  $\forall f \in \mathcal{F}, id_f \in \text{Outs}(\Delta) \text{ s.t. } \gamma(f) = id_f, s'.ex(f) = \sigma'(id_f).$
7.  $\forall t \in T, id_t \in \text{Comps}(\Delta) \text{ s.t. } \gamma(t) = id_t, t \in \text{Firable}(s') \Leftrightarrow \sigma'(id_t)("s\_firable") = \text{true}.$
8.  $\forall t \in T, id_t \in \text{Comps}(\Delta) \text{ s.t. } \gamma(t) = id_t, t \notin \text{Firable}(s') \Leftrightarrow \sigma'(id_t)("s\_firable") = \text{false}.$
9.  $\forall t \in T, id_t \in \text{Comps}(\Delta) \text{ s.t. } \gamma(t) = id_t, t \in \text{Fired}(s') \Leftrightarrow \sigma'(id_t)("fired") = \text{true}.$
10.  $\forall t \in T, id_t \in \text{Comps}(\Delta) \text{ s.t. } \gamma(t) = id_t, t \notin \text{Fired}(s') \Leftrightarrow \sigma'(id_t)("fired") = \text{false}.$
11.  $\forall p \in P, id_p \in \text{Comps}(\Delta) \text{ s.t. } \gamma(p) = id_p, \sum_{t \in \text{Fired}(s')} pre(p, t) = \sigma'(id_p)("s\_output\_token\_sum").$
12.  $\forall p \in P, id_p \in \text{Comps}(\Delta) \text{ s.t. } \gamma(p) = id_p, \sum_{t \in \text{Fired}(s')} post(t, p) = \sigma'(id_p)("s\_input\_token\_sum").$

Each point is proved by a separate lemma:

- Apply Lemma **Falling Edge Equal Marking** to solve 1.
- Apply Lemma **Falling Edge Equal Time Counters** to solve 2.
- Apply Lemma **Falling Edge Equal Output Token Sum** to solve 11.
- Apply Lemma **Falling Edge Equal Input Token Sum** to solve 12.

□

### 1.6.1 Falling Edge and marking

**Lemma 5** (Falling Edge Equal Marking). *For all  $sitpn, d, \gamma, \Delta, \sigma_e, E_c, E_p, \tau, s, s', \sigma, \sigma_i, \sigma_\downarrow, \sigma'$  that verify the hypotheses of Def. 1, then  $\forall p \in P, id_p \in Comps(\Delta)$  s.t.  $\gamma(p) = id_p, s'.M(p) = \sigma'(id_p)("s\_marking")$ .*

*Proof.* Given a  $p \in P$  and an  $id \in Comps(\Delta)$  s.t.  $\gamma(p) = id_p$ , let us show

$$s'.M(p) = \sigma'(id_p)("s\_marking").$$

By definition of  $E_c, \tau \vdash sitpn, s \xrightarrow{\downarrow} s'$ :

$$s.M(p) = s'.M(p) \quad (1.1)$$

By property of the  $Inject_\downarrow$  relation, the  $\mathcal{H}$ -VHDL falling edge relation, the stabilize relation and  $comp(id_p, "place", gm_p, ipm_p, opm_p) \in d.cs$ :

$$\sigma'(id_p)("s\_marking") = \sigma(id_p)("s\_marking") \quad (1.2)$$

Rewriting the goal with (1.1) and (1.2):  $s.M(p) = \sigma(id_p)("s\_marking").$

By definition of  $\gamma, E_c, \tau \vdash s \xrightarrow{\downarrow} s'$ :  $s.M(p) = \sigma(id_p)("s\_marking").$

□

**Lemma 6** (Falling Edge Equal Output Token Sum). *For all  $sitpn, d, \gamma, \Delta, \sigma_e, E_c, E_p, \tau, s, s', \sigma, \sigma_i, \sigma_\downarrow, \sigma'$  that verify the hypotheses of Def. 1, then  $\forall p, id_p$  s.t.  $\gamma(p) = id_p, \sum_{t \in Fired(s')} pre(p, t) = \sigma'(id_p)("s\_output\_token\_sum")$ .*

*Proof.* Given a  $p \in P$  and an  $id_p \in Comps(\Delta)$ , let us show

$$\sum_{t \in Fired(s')} pre(p, t) = \sigma'(id_p)("s\_output\_token\_sum").$$

By definition of  $id_p$ , there exist  $gm_p, ipm_p, opm_p$  s.t.  $comp(id_p, "place", gm_p, ipm_p, opm_p) \in d.cs$ .

By property of the stabilize relation and  $comp(id_p, "place", gm_p, ipm_p, opm_p) \in d.cs$ :

$$\sigma'(id_p)("sots") = \sum_{i=0}^{\Delta(id_p)("oan")-1} \begin{cases} \sigma'(id_p)("oaw")[i] & \text{if } (\sigma'(id_p)("otf"))[i] \\ & . \sigma'(id_p)("oat")[i] = \text{BASIC} \\ 0 & \text{otherwise} \end{cases} \quad (1.3)$$

Rewriting the goal with (1.3):

$$\sum_{t \in Fired(s')} pre(p, t) = \sum_{i=0}^{\Delta(id_p)("oan")-1} \begin{cases} \sigma'(id_p)("oaw")[i] & \text{if } (\sigma'(id_p)("otf"))[i] \\ & . \sigma'(id_p)("oat")[i] = \text{BASIC} \\ 0 & \text{otherwise} \end{cases}$$

Let us unfold the definition of the left sum term:

$$\sum_{t \in \text{Fired}(s')} \begin{cases} \omega & \text{if } \text{pre}(p, t) = (\omega, \text{basic}) \\ 0 & \text{otherwise} \end{cases} = \sum_{i=0}^{\Delta(id_p)("oan")-1} \begin{cases} \sigma'(id_p)("oaw")[i] & \text{if } (\sigma'(id_p)("otf")[i] \cdot \sigma'(id_p)("oat")[i] = \text{BASIC}) \\ 0 & \text{otherwise} \end{cases}$$

To ease the reading, let us define functions  $f \in \text{Fired}(s') \rightarrow \mathbb{N}$  and  $g \in [0, |\text{output}(p)| - 1] \rightarrow \mathbb{N}$  s.t.

$$f(t) = \begin{cases} \omega & \text{if } \text{pre}(p, t) = (\omega, \text{basic}) \\ 0 & \text{otherwise} \end{cases} \quad \text{and } g(i) = \begin{cases} \sigma'(id_p)("oaw")[i] & \text{if } (\sigma'(id_p)("otf")[i] \cdot \sigma'(id_p)("oat")[i] = \text{BASIC}) \\ 0 & \text{otherwise} \end{cases}$$

Then, the goal is:

$$\sum_{t \in \text{Fired}(s')} f(t) = \sum_{i=0}^{\Delta(id_p)("oan")-1} g(i)$$

Let us perform case analysis on  $\text{output}(p)$ ; there are two cases:

1.  $\text{output}(p) = \emptyset$ :

By construction,  $\langle \text{output\_arcs\_number} \Rightarrow 1 \rangle \in gm_p$ ,  $\langle \text{output\_arcs\_types}(0) \Rightarrow \text{BASIC} \rangle \in ipm_p$ ,  $\langle \text{output\_transitions\_fired}(0) \Rightarrow \text{true} \rangle \in ipm_p$ , and  $\langle \text{output\_arcs\_weights}(0) \Rightarrow 0 \rangle \in ipm_p$ .

By property of the elaboration relation and  $\text{comp}(id_p, "place", gm_p, ipm_p, opm_p) \in d.cs$ :

$$\Delta(id_p)("oan") = 1 \tag{1.4}$$

By property of the stabilize relation and  $\text{comp}(id_p, "place", gm_p, ipm_p, opm_p) \in d.cs$ :

$$\sigma'(id_p)("oat")[0] = \text{BASIC} \tag{1.5}$$

$$\sigma'(id_p)("otf")[0] = \text{true} \tag{1.6}$$

$$\sigma'(id_p)("oaw")[0] = 0 \tag{1.7}$$

By property of  $\text{output}(p) = \emptyset$ :

$$\sum_{t \in \text{Fired}(s')} \begin{cases} \omega & \text{if } \text{pre}(p, t) = (\omega, \text{basic}) \\ 0 & \text{otherwise} \end{cases} = 0 \tag{1.8}$$

Rewriting the goal with (1.4), (1.5), (1.6), (1.7) and (1.8), **tautology**.

2.  $\text{output}(p) \neq \emptyset$ :

By construction,  $\langle \text{output\_arcs\_number} \Rightarrow |\text{output}(p)| \rangle \in gm_p$ , and by property of the elaboration relation:

$$\Delta(id_p)("oan") = |\text{output}(p)| \tag{1.9}$$

Rewriting the goal with (1.9):  $\sum_{t \in \text{Fired}(s')} f(t) = \sum_{i=0}^{|\text{output}(p)|-1} g(i).$

Let us reason by induction on the right sum term of the goal.

- **BASE CASE:**

In that case,  $0 > |\text{output}| - 1$  and  $\sum_{i=0}^{|\text{output}(p)|-1} g(i) = 0.$

As  $0 > |\text{output}| - 1$ , then  $|\text{output}(p)| = 0$ , thus contradicting  $\text{output}(p) \neq \emptyset$ .

- **INDUCTION CASE:**

In that case,  $0 \leq |\text{output}(p)| - 1.$

$$\forall F \subseteq \text{Fired}(s'), g(0) + \sum_{t \in F} f(t) = g(0) + \sum_{i=1}^{|\text{output}(p)|-1} g(i)$$

$$\sum_{t \in \text{Fired}(s')} f(t) = g(0) + \sum_{i=1}^{|\text{output}(p)|-1} g(i)$$

By definition of  $g$ :

$$g(0) = \begin{cases} \sigma'(id_p)("oaw")[0] & \text{if } (\sigma'(id_p)("otf")[0] \cdot \sigma'(id_p)("oat")[0] = \text{BASIC}) \\ 0 & \text{otherwise} \end{cases} \quad (1.10)$$

Let us perform case analysis on the value of  $\sigma'(id_p)("otf")[0] \cdot \sigma'(id_p)("oat")[0] = \text{BASIC}$ ; there are two cases:

(a)  $(\sigma'(id_p)("otf")[0] \cdot \sigma'(id_p)("oat")[0] = \text{BASIC}) = \text{false}$ :

In that case,  $g(0) = 0$ , and then we can apply the induction hypothesis with  $F =$

$\text{Fired}(s')$  to solve the goal:  $\sum_{t \in \text{Fired}(s')} f(t) = \sum_{i=1}^{|\text{output}(p)|-1} g(i).$

(b)  $(\sigma'(id_p)("otf")[0] \cdot \sigma'(id_p)("oat")[0] = \text{BASIC}) = \text{true}$ :

In that case,  $g(0) = \sigma'(id_p)("oaw")[0]$ ,  $\sigma'(id_p)("otf")[0] = \text{true}$  and  $\sigma'(id_p)("oat")[0] = \text{BASIC}.$

By construction, there exist a  $t \in \text{output}(t)$ ,  $id_t \in \text{Comps}(\Delta)$  s.t.  $\gamma(t) = id_t$ . Let us take such a  $t \in \text{output}(p).$

By definition of  $id_t$ , there exist  $gm_t, ipm_t, opm_t$  s.t.  $\text{comp}(id_t, "transition", gm_t, ipm_t, opm_t) \in d.cs.$

As  $t \in \text{output}(p)$ , there exist  $\omega \in \mathbb{N}^*$  and  $a \in \{\text{BASIC}, \text{TEST}, \text{INHIB}\}$  s.t.  $\text{pre}(p, t) = (\omega, a).$  Let us take an  $\omega$  and  $a$  s.t.  $\text{pre}(p, t) = (\omega, a).$

By construction,  $\langle \text{output\_arcs\_types}(0) \Rightarrow a \rangle \in ipm_p,$

$\langle \text{output\_arcs\_weights}(0) \Rightarrow \omega \rangle \in ipm_p,$  and there exists  $id_{ft} \in \text{Sigs}(\Delta)$  s.t.

$\langle \text{fired} \Rightarrow id_{ft} \rangle \in opm_t$  and  $\langle \text{output\_transitions\_fired}(0) \Rightarrow id_{ft} \rangle \in ipm_p$



By property of the stabilize relation,  $\sigma'(id_p)("oat")[0] = \text{BASIC}$  and  $\langle \text{output\_arcs\_types}(0) \Rightarrow a \rangle \in ipm_p$ :

$$pre(p, t) = (\omega, \text{basic}) \quad (1.11)$$

By property of the stabilize relation,  $\langle \text{fired} \Rightarrow id_{ft} \rangle \in opm_t$ ,  $\langle \text{output\_transitions\_fired}(0) \Rightarrow id_{ft} \rangle \in ipm_p$  and  $\sigma'(id_p)("otf")[0] = \text{true}$ :

$$\sigma'(id_t)("fired") = \text{true} \quad (1.12)$$

Appealing to Lemma ??, we know  $t \in \text{Fired}(s')$ .

As  $t \in \text{Fired}(s')$ , we can rewrite the left sum term of the goal as follows:

$$f(t) + \sum_{t' \in \text{Fired}(s') \setminus \{t\}} f(t') = g(0) + \sum_{i=1}^{|\text{output}(p)|-1} g(i)$$

We know that  $g(0) = \sigma'(id_p)("oaw")[0]$ , and by property of the stabilize relation and  $\langle \text{output\_arcs\_weights}(0) \Rightarrow \omega \rangle \in ipm_p$ :

$$\sigma'(id_p)("oaw")[0] = \omega \quad (1.13)$$

Rewriting the goal with (1.13):

$$f(t) + \sum_{t' \in \text{Fired}(s') \setminus \{t\}} f(t') = \omega + \sum_{i=1}^{|\text{output}(p)|-1} g(i)$$

By definition of  $f$ , and as  $pre(p, t) = (\omega, \text{basic})$ , then  $f(t) = \omega$ ; thus, rewriting the goal:

$$\omega + \sum_{t' \in \text{Fired}(s') \setminus \{t\}} f(t') = \omega + \sum_{i=1}^{|\text{output}(p)|-1} g(i)$$

Then, knowing that  $g(0) = \omega$ , we can apply the induction hypothesis with  $F =$

$$\text{Fired}(s') \setminus \{t\}: g(0) + \sum_{t' \in \text{Fired}(s') \setminus \{t\}} f(t') = g(0) + \sum_{i=1}^{|\text{output}(p)|-1} g(i).$$

□

**Lemma 7** (Falling Edge Equal Input Token Sum). *For all  $sitpn, d, \gamma, \Delta, \sigma_e, E_c, E_p, \tau, s, s', \sigma, \sigma_i, \sigma_\downarrow, \sigma'$  that verify the hypotheses of Def. 1, then  $\forall p, id_p$  s.t.  $\gamma(p) = id_p$ ,  $\sum_{t \in \text{Fired}(s')} post(t, p) = \sigma'_p("s\_input\_token\_sum")$ .*

*Proof.* Given a  $p \in P$  and an  $id_p \in \text{Comps}(\Delta)$ , let us show

$$\sum_{t \in \text{Fired}(s')} post(t, p) = \sigma'(id_p)("s\_input\_token\_sum").$$

By definition of  $id_p$ , there exist  $gm_p, ipm_p, opm_p$  s.t.  $\text{comp}(id_p, "place", gm_p, ipm_p, opm_p) \in d.cs$ .

By property of the stabilize relation and  $\text{comp}(id_p, "place", gm_p, ipm_p, opm_p) \in d.cs$ :

$$\sigma'(id_p)("sits") = \sum_{i=0}^{\Delta(id_p)("ian")-1} \begin{cases} \sigma'(id_p)("iaw")[i] & \text{if } \sigma'(id_p)("itf")[i] \\ 0 & \text{otherwise} \end{cases} \quad (1.14)$$

Rewriting the goal with (1.14):

$$\sum_{t \in \text{Fired}(s')} \text{post}(t, p) = \sum_{i=0}^{\Delta(id_p)("ian")-1} \begin{cases} \sigma'(id_p)("iaw")[i] & \text{if } \sigma'(id_p)("otf")[i] \\ 0 & \text{otherwise} \end{cases}$$

Let us unfold the definition of the left sum term:

$$\begin{aligned} \sum_{t \in \text{Fired}(s')} \begin{cases} \omega & \text{if } \text{post}(t, p) = \omega \\ 0 & \text{otherwise} \end{cases} \\ = \\ \sum_{i=0}^{\Delta(id_p)("ian")-1} \begin{cases} \sigma'(id_p)("iaw")[i] & \text{if } \sigma'(id_p)("itf")[i] \\ 0 & \text{otherwise} \end{cases} \end{aligned}$$

Let us perform case analysis on  $\text{input}(p)$ ; there are two cases:

1.  $\text{input}(p) = \emptyset$ :

By construction,  $\langle \text{input\_arcs\_number} \Rightarrow 1 \rangle \in gm_p$ ,  $\langle \text{input\_transitions\_fired}(0) \Rightarrow \text{true} \rangle \in ipm_p$ , and  $\langle \text{input\_arcs\_weights}(0) \Rightarrow 0 \rangle \in ipm_p$ .

By property of the elaboration relation and  $\text{comp}(id_p, "place", gm_p, ipm_p, opm_p) \in d.cs$ :

$$\Delta(id_p)("ian") = 1 \quad (1.15)$$

By property of the stabilize relation and  $\text{comp}(id_p, "place", gm_p, ipm_p, opm_p) \in d.cs$ :

$$\sigma'(id_p)("itf")[0] = \text{true} \quad (1.16)$$

$$\sigma'(id_p)("iaw")[0] = 0 \quad (1.17)$$

By property of  $\text{input}(p) = \emptyset$ :

$$\sum_{t \in \text{Fired}(s')} \begin{cases} \omega & \text{if } \text{post}(t, p) = \omega \\ 0 & \text{otherwise} \end{cases} = 0 \quad (1.18)$$

Rewriting the goal with (1.15), (1.16), (1.17), and (1.18), and simplifying the goal, **tautology**.

2.  $\text{input}(p) \neq \emptyset$ :

By construction,  $\langle \text{input\_arcs\_number} \Rightarrow |\text{input}(p)| \rangle \in gm_p$ , and by property of the elaboration relation:

$$\Delta(id_p)("ian") = |\text{input}(p)| \quad (1.19)$$

To ease the reading, let us define functions  $f \in \text{Fired}(s') \rightarrow \mathbb{N}$  and  $g \in [0, |\text{input}(p)| - 1] \rightarrow \mathbb{N}$  s.t.  $f(t) = \begin{cases} \omega & \text{if } \text{post}(t, p) = \omega \\ 0 & \text{otherwise} \end{cases}$  and

$$g(i) = \begin{cases} \sigma'(id_p)("iaw")[i] & \text{if } \sigma'(id_p)("itf")[i] \\ 0 & \text{otherwise} \end{cases}$$

Then, the goal is:

$$\sum_{t \in \text{Fired}(s')} f(t) = \sum_{i=0}^{\Delta(id_p)("ian")-1} g(i)$$

Rewriting the goal with (1.19):

$$\sum_{t \in \text{Fired}(s')} f(t) = \sum_{i=0}^{|input(p)|-1} g(i).$$

Let us reason by induction on the right sum term of the goal.

• **BASE CASE:**

In that case,  $0 > |input(p)| - 1$  and  $\sum_{i=0}^{|input(p)|-1} g(i) = 0$ .

As  $0 > |input(p)| - 1$ , then  $|input(p)| = 0$ , thus **contradicting  $input(p) \neq \emptyset$ .**

• **INDUCTION CASE:**

In that case,  $0 \leq |input(p)| - 1$ .

$$\forall F \subseteq \text{Fired}(s'), g(0) + \sum_{t \in F} f(t) = g(0) + \sum_{i=1}^{|input(p)|-1} g(i)$$

$$\sum_{t \in \text{Fired}(s')} f(t) = g(0) + \sum_{i=1}^{|input(p)|-1} g(i)$$

By definition of  $g$ :

$$g(0) = \begin{cases} \sigma'(id_p)("iaw")[0] & \text{if } \sigma'(id_p)("itf")[0] \\ 0 & \text{otherwise} \end{cases} \quad (1.20)$$

Let us perform case analysis on the value of  $\sigma'(id_p)("itf")[0]$ ; there are two cases:

(a)  $\sigma'(id_p)("itf")[0] = \text{false}$ :

In that case,  $g(0) = 0$ , and then we can apply the induction hypothesis with  $F =$

$\text{Fired}(s')$  to solve the goal:

$$\sum_{t \in \text{Fired}(s')} f(t) = \sum_{i=1}^{|input(p)|-1} g(i).$$

(b)  $\sigma'(id_p)("itf")[0] = \text{true}$ :

In that case,  $g(0) = \sigma'(id_p)("iaw")[0]$  and  $\sigma'(id_p)("itf")[0] = \text{true}$ .

By construction, there exist a  $t \in input(p)$ ,  $id_t \in Comps(\Delta)$  s.t.  $\gamma(t) = id_t$ . Let us take such a  $t \in input(p)$ .

By definition of  $id_t$ , there exist  $gm_t, ipm_t, opm_t$  s.t.  $\text{comp}(id_t, "transition", gm_t, ipm_t, opm_t) \in d.cs$ .

As  $t \in input(p)$ , there exist  $\omega \in \mathbb{N}^*$  s.t.  $\text{post}(t, p) = \omega$ . Let us take an  $\omega$  s.t.  $\text{post}(t, p) = \omega$ .

By construction,  $\langle input\_arcs\_weights(0) \Rightarrow \omega \rangle \in ipm_p$ , and there exists  $id_{ft} \in Sigs(\Delta)$  s.t.  $\langle \text{fired} \Rightarrow id_{ft} \rangle \in opm_t$  and  $\langle input\_transitions\_fired(0) \Rightarrow id_{ft} \rangle \in ipm_p$

By property of the stabilize relation and  $\langle input\_arcs\_types(0) \Rightarrow a \rangle \in ipm_p$ :

$$\text{post}(t, p) = \omega \quad (1.21)$$

By property of the stabilize relation,  $\langle \text{fired} \Rightarrow \text{id}_{ft} \rangle \in \text{opm}_t$ ,  
 $\langle \text{input\_transitions\_fired}(0) \Rightarrow \text{id}_{ft} \rangle \in \text{ipm}_p$  and  $\sigma'(\text{id}_p)("itf")[0] = \text{true}$ :

$$\sigma'(\text{id}_t)("fired") = \text{true} \quad (1.22)$$

Appealing to Lemma ?? and (1.22), we know  $t \in \text{Fired}(s')$ .

As  $t \in \text{Fired}(s')$ , we can rewrite the left sum term of the goal as follows:

$$f(t) + \sum_{t' \in \text{Fired}(s') \setminus \{t\}} f(t') = g(0) + \sum_{i=1}^{|\text{input}(p)|-1} g(i)$$

We know that  $g(0) = \sigma'(\text{id}_p)("iaw")[0]$ , and by property of the stabilize relation and  $\langle \text{input\_arcs\_weights}(0) \Rightarrow \omega \rangle \in \text{ipm}_p$ :

$$\sigma'(\text{id}_p)("iaw")[0] = \omega \quad (1.23)$$

Rewriting the goal with (1.23):

$$f(t) + \sum_{t' \in \text{Fired}(s') \setminus \{t\}} f(t') = \omega + \sum_{i=1}^{|\text{input}(p)|-1} g(i)$$

By definition of  $f$ , and as  $\text{post}(t, p) = \omega$ , then  $f(t) = \omega$ ; thus, rewriting the goal:

$$\omega + \sum_{t' \in \text{Fired}(s') \setminus \{t\}} f(t') = \omega + \sum_{i=1}^{|\text{input}(p)|-1} g(i)$$

Then, knowing that  $g(0) = \omega$ , we can apply the induction hypothesis with  $F =$

$$\text{Fired}(s') \setminus \{t\}: g(0) + \sum_{t' \in \text{Fired}(s') \setminus \{t\}} f(t') = g(0) + \sum_{i=1}^{|\text{input}(p)|-1} g(i).$$

□

### 1.6.2 Falling edge and time counters

**Lemma 8** (Falling Edge Equal Time Counters). *For all  $\text{sitpn}, d, \gamma, \Delta, \sigma_e, E_c, E_p, \tau, s, s', \sigma, \sigma_i, \sigma_\downarrow, \sigma'$  that verify the hypotheses of Def. 1, then  $\forall t \in T_i, \text{id}_t \in \text{Comps}(\Delta)$  s.t.  $\gamma(t) = \text{id}_t$ ,*

$$\begin{aligned} &(\text{upper}(I_s(t)) = \infty \wedge s'.I(t) \leq \text{lower}(I_s(t)) \Rightarrow s'.I(t) = \sigma'(\text{id}_t)("s\_time\_counter")) \\ &\wedge (\text{upper}(I_s(t)) = \infty \wedge s'.I(t) > \text{lower}(I_s(t)) \Rightarrow \sigma'(\text{id}_t)("s\_time\_counter") = \text{lower}(I_s(t))) \\ &\wedge (\text{upper}(I_s(t)) \neq \infty \wedge s'.I(t) > \text{upper}(I_s(t)) \Rightarrow \sigma'(\text{id}_t)("s\_time\_counter") = \text{upper}(I_s(t))) \\ &\wedge (\text{upper}(I_s(t)) \neq \infty \wedge s'.I(t) \leq \text{upper}(I_s(t)) \Rightarrow s'.I(t) = \sigma'(\text{id}_t)("s\_time\_counter")). \end{aligned}$$

*Proof.* Given a  $t \in T_i$  and an  $\text{id}_t \in \text{Comps}(\Delta)$  s.t.  $\gamma(t) = \text{id}_t$ , let us show

$$\begin{aligned} &(\text{upper}(I_s(t)) = \infty \wedge s'.I(t) \leq \text{lower}(I_s(t)) \Rightarrow s'.I(t) = \sigma'(\text{id}_t)("s\_time\_counter")) \\ &\wedge (\text{upper}(I_s(t)) = \infty \wedge s'.I(t) > \text{lower}(I_s(t)) \Rightarrow \sigma'(\text{id}_t)("s\_time\_counter") = \text{lower}(I_s(t))) \\ &\wedge (\text{upper}(I_s(t)) \neq \infty \wedge s'.I(t) > \text{upper}(I_s(t)) \Rightarrow \sigma'(\text{id}_t)("s\_time\_counter") = \text{upper}(I_s(t))) \\ &\wedge (\text{upper}(I_s(t)) \neq \infty \wedge s'.I(t) \leq \text{upper}(I_s(t)) \Rightarrow s'.I(t) = \sigma'(\text{id}_t)("s\_time\_counter")) \end{aligned}$$

By definition of  $\text{id}_t$ , there exist  $gm_t, ipm_t, opm_t$  s.t.  $\text{comp}(\text{id}_t, "transition", gm_t, ipm_t, opm_t) \in d.cs$ .

By property of the elaboration,  $\text{Inject}_\downarrow$ ,  $\mathcal{H}$ -VHDL rising edge and stabilize relations, and  $\text{comp}(id_t, \text{"transition"}, gm_t, ipm_t, opm_t) \in d.cs$ :

$$\begin{aligned} \sigma(id_t)(\text{"se"}) = \text{true} \wedge \Delta(id_t)(\text{"tt"}) \neq \text{NOT\_TEMPORAL} \wedge \sigma(id_t)(\text{"srtc"}) = \text{false} \\ \wedge \sigma(id_t)(\text{"stc"}) < \Delta(id_t)(\text{"mtc"}) \Rightarrow \sigma'(id_t)(\text{"stc"}) = \sigma(id_t)(\text{"stc"}) + 1 \end{aligned} \quad (1.24)$$

$$\begin{aligned} \sigma(id_t)(\text{"se"}) = \text{true} \wedge \Delta(id_t)(\text{"tt"}) \neq \text{NOT\_TEMPORAL} \wedge \sigma(id_t)(\text{"srtc"}) = \text{false} \\ \wedge \sigma(id_t)(\text{"stc"}) \geq \Delta(id_t)(\text{"mtc"}) \Rightarrow \sigma'(id_t)(\text{"stc"}) = \sigma(id_t)(\text{"stc"}) \end{aligned} \quad (1.25)$$

$$\begin{aligned} \sigma(id_t)(\text{"se"}) = \text{true} \wedge \Delta(id_t)(\text{"tt"}) \neq \text{NOT\_TEMPORAL} \\ \wedge \sigma(id_t)(\text{"srtc"}) = \text{true} \Rightarrow \sigma'(id_t)(\text{"stc"}) = 1 \end{aligned} \quad (1.26)$$

$$\sigma(id_t)(\text{"se"}) = \text{false} \vee \Delta(id_t)(\text{"tt"}) = \text{NOT\_TEMPORAL} \Rightarrow \sigma'(id_t)(\text{"stc"}) = 0 \quad (1.27)$$

Then, there are 4 points to show:

$$1. \boxed{\text{upper}(I_s(t)) = \infty \wedge s'.I(t) \leq \text{lower}(I_s(t)) \Rightarrow s'.I(t) = \sigma'(id_t)(\text{"s\_time\_counter"})}$$

Assuming  $\text{upper}(I_s(t)) = \infty$  and  $s'.I(t) \leq \text{lower}(I_s(t))$ , let us show

$$\boxed{s'.I(t) = \sigma'(id_t)(\text{"s\_time\_counter"})}.$$

Case analysis on  $t \in \text{Sens}(s.M)$ ; there are two cases:

(a)  $t \notin \text{Sens}(s.M)$ :

By definition of  $\gamma, E_c, \tau \vdash s \downarrow \sigma$ :

$$\sigma(id_t)(\text{"se"}) = \text{false} \quad (1.28)$$

Thanks to (1.27) and (1.28):

$$\sigma'(id_t)(\text{"stc"}) = 0 \quad (1.29)$$

By definition of  $E_c, \tau \vdash s \xrightarrow{\downarrow} s'$ :

$$s'.I(t) = 0 \quad (1.30)$$

Rewriting the goal with (1.29) and (1.30): **tautology.**

(b)  $t \in \text{Sens}(s.M)$ :

By definition of  $\gamma, E_c, \tau \vdash s \uparrow \sigma$ :

$$\sigma(id_t)(\text{"se"}) = \text{true} \quad (1.31)$$

By construction, and as  $\text{upper}(I_s(t)) = \infty$ ,  $\langle \text{transition\_type} \Rightarrow \text{TEMP\_A\_INF} \rangle \in gm_t$ .

By property of the elaboration relation:

$$\Delta(id_t)(\text{"tt"}) = \text{TEMP\_A\_INF} \quad (1.32)$$

Case analysis on  $s.reset_t(t)$ ; there are two cases:

i.  $s.reset_t(t) = \text{true}$ :

By definition of  $\gamma, E_c, \tau \vdash s \overset{\uparrow}{\sim} \sigma$ :

$$\sigma(id_t)("srtc") = \text{true} \quad (1.33)$$

Thanks to (1.26), (1.31), (1.32) and (1.33):

$$\sigma'(id_t)("stc") = 1 \quad (1.34)$$

By definition of  $E_c, \tau \vdash s \overset{\downarrow}{\rightarrow} s'$ :

$$s'.I(t) = 1 \quad (1.35)$$

Rewriting the goal with (1.34) and (1.35): **tautology.**

ii.  $s.reset_t(t) = \text{false}$ : By definition of  $\gamma, E_c, \tau \vdash s \overset{\uparrow}{\sim} \sigma$ :

$$\sigma(id_t)("srtc") = \text{false} \quad (1.36)$$

As  $upper(I_s(t)) = \infty$ , there exists an  $a \in \mathbb{N}^*$  s.t.  $I_s(t) = [a, \infty]$ . Let us take such an  $a \in \mathbb{N}^*$ . By construction,  $\langle \text{maximal\_time\_counter} \Rightarrow a \rangle \in gm_t$ , and by property of the elaboration relation:

$$\Delta(id_t)("mtc") = a \quad (1.37)$$

By definition of  $E_c, \tau \vdash s \overset{\downarrow}{\rightarrow} s'$ , and knowing that  $t \in \text{Sens}(s.M)$  and  $s.reset_t(t) = \text{false}$  and  $upper(I_s(t)) = \infty$ :

$$s'.I(t) = s.I(t) + 1 \quad (1.38)$$

Rewriting the goal with (1.38):  $s.I(t) + 1 = \sigma'(id_t)("stc")$ .

We assumed that  $s'.I(t) \leq lower(I_s(t))$ , and as  $s'.I(t) = s.I(t) + 1$ , then  $s.I(t) + 1 \leq lower(I_s(t))$ , then  $s.I(t) < lower(I_s(t))$ , then  $s.I(t) < a$  since  $a = lower(I_s(t))$ .

By definition of  $\gamma, E_c, \tau \vdash s \overset{\uparrow}{\sim} \sigma$ , and knowing that  $s.I(t) < lower(I_s(t))$  and  $upper(I_s(t)) = \infty$ :

$$s.I(t) = \sigma(id_t)("stc") \quad (1.39)$$

Thanks to (1.37), (1.39) and  $s.I(t) < a$ :

$$\sigma(id_t)("stc") < \Delta(id_t)("mtc") \quad (1.40)$$

Thanks to (1.24), (1.40), (1.36) and (1.31):

$$\sigma'(id_t)("stc") = \sigma(id_t)("stc") + 1 \quad (1.41)$$

Rewriting the goal with (1.41) and (1.39): **tautology.**

2.  $upper(I_s(t)) = \infty \wedge s'.I(t) > lower(I_s(t)) \Rightarrow \sigma'(id_t)("s\_time\_counter") = lower(I_s(t))$ .

Assuming that  $upper(I_s(t)) = \infty$  and  $s'.I(t) > lower(I_s(t))$ , let us show

$$\sigma'(id_t)("s\_time\_counter") = lower(I_s(t)).$$

As  $upper(I_s(t)) = \infty$ , there exists an  $a \in \mathbb{N}^*$  s.t.  $I_s(t) = [a, \infty]$ . Let us take such an  $a \in \mathbb{N}^*$ . By construction,  $\langle \text{maximal\_time\_counter} \Rightarrow a \rangle \in gm_t$ , and  $\langle \text{transition\_type} \Rightarrow \text{TEMP\_A\_INF} \rangle \in gm_t$  by property of the elaboration relation:

$$\Delta(id_t)("mtc") = a \quad (1.42)$$

$$\Delta(id_t)("tt") = \text{TEMP\_A\_INF} \quad (1.43)$$

Case analysis on  $t \in \text{Sens}(s.M)$ :

(a)  $t \notin \text{Sens}(s.M)$ :

By definition of  $E_c, \tau \vdash s \xrightarrow{\downarrow} s'$ , and knowing that  $t \in \text{Sens}(s.M)$ , then  $s'.I(t) = 0$ . Since  $lower(I_s(t)) \in \mathbb{N}^*$ , then  $lower(I_s(t)) > 0$ .

Contradicts  $s'.I(t) > lower(I_s(t))$ .

(b)  $t \in \text{Sens}(s.M)$ :

By definition of  $\gamma, E_c, \tau \vdash s \xrightarrow{\uparrow} \sigma$  and  $t \in \text{Sens}(s.M)$ :

$$\sigma(id_t)("se") = \text{true} \quad (1.44)$$

Case analysis on  $s.\text{reset}_t(t)$ ; there are two cases:

i.  $s.\text{reset}_t(t) = \text{true}$ :

By definition of  $E_c, \tau \vdash s \xrightarrow{\downarrow} s'$ :  $s'.I(t) = 1$ .

We assumed that  $s'.I(t) > lower(I_s(t))$ , then  $1 > lower(I_s(t))$ .

Contradicts  $lower(I_s(t)) > 0$ .

ii.  $s.\text{reset}_t(t) = \text{false}$ :

By property of  $\gamma, E_c, \tau \vdash s \xrightarrow{\uparrow} \sigma$  and  $s.\text{reset}_t(t) = \text{false}$ :

$$\sigma(id_t)("srtc") = \text{false} \quad (1.45)$$

By definition of  $E_c, \tau \vdash s \xrightarrow{\downarrow} s'$ , and knowing that  $s'.I(t) > lower(I_s(t))$ :

$$\begin{aligned} s'.I(t) &= s.I(t) + 1 \Rightarrow s.I(t) + 1 > lower(I_s(t)) \\ &\Rightarrow s.I(t) \geq lower(I_s(t)) \end{aligned} \quad (1.46)$$

Case analysis on  $s.I(t) \geq lower(I_s(t))$ :

A.  $s.I(t) > lower(I_s(t))$ :  $\sigma'(id_t)("stc") = lower(I_s(t))$ .

By definition of  $\gamma, E_c, \tau \vdash s \xrightarrow{\uparrow} \sigma$ :

$$\sigma(id_t)("stc") = lower(I_s(t)) \quad (1.47)$$

Thanks to (1.25):

$$\sigma'(id_t)("stc") = \sigma(id_t)("stc") \quad (1.48)$$

Rewriting the goal with (1.47) and (1.55): tautology.

$$\text{B. } s.I(t) = \text{lower}(I_s(t)): \boxed{\sigma'(id_t)("stc") = \text{lower}(I_s(t))}.$$

By definition of  $\gamma, E_c, \tau \vdash s \overset{\uparrow}{\sim} \sigma$ :

$$s.I(t) = \sigma(id_t)("stc") \quad (1.49)$$

Thanks to (1.25):

$$\sigma'(id_t)("stc") = \sigma(id_t)("stc") \quad (1.50)$$

Rewriting the goal with (1.57), (1.56) and  $s.I(t) = \text{lower}(I_s(t))$ : **tautology.**

$$3. \boxed{\text{upper}(I_s(t)) \neq \infty \wedge s'.I(t) > \text{upper}(I_s(t)) \Rightarrow \sigma'(id_t)("s\_time\_counter") = \text{upper}(I_s(t))}.$$

Assuming that  $\text{upper}(I_s(t)) \neq \infty$  and  $s'.I(t) > \text{upper}(I_s(t))$ , let us show

$$\boxed{\sigma'(id_t)("s\_time\_counter") = \text{upper}(I_s(t))}.$$

As  $\text{upper}(I_s(t)) \neq \infty$ , there exists an  $a \in \mathbb{N}^*$ , and a  $b \in \mathbb{N}^*$  s.t.  $I_s(t) = [a, b]$ . Let us take such an  $a$  and  $b$ . By construction, there exists  $tt \in \{$

Case analysis on  $t \in \text{Sens}(s.M)$ :

(a)  $t \notin \text{Sens}(s.M)$ :

By definition of  $E_c, \tau \vdash s \overset{\downarrow}{\rightarrow} s'$ , and knowing that  $t \in \text{Sens}(s.M)$ , then  $s'.I(t) = 0$ . Since  $\text{upper}(I_s(t)) \in \mathbb{N}^*$ , then  $\text{upper}(I_s(t)) > 0$ .

**Contradicts  $s'.I(t) > \text{upper}(I_s(t))$ .**

(b)  $t \in \text{Sens}(s.M)$ :

By definition of  $\gamma, E_c, \tau \vdash s \overset{\uparrow}{\sim} \sigma$  and  $t \in \text{Sens}(s.M)$ :

$$\sigma(id_t)("se") = \text{true} \quad (1.51)$$

Case analysis on  $s.\text{reset}_t(t)$ ; there are two cases:

i.  $s.\text{reset}_t(t) = \text{true}$ :

By definition of  $E_c, \tau \vdash s \overset{\downarrow}{\rightarrow} s'$ :  $s'.I(t) = 1$ .

We assumed that  $s'.I(t) > \text{upper}(I_s(t))$ , then  $1 > \text{upper}(I_s(t))$ .

**Contradicts  $\text{upper}(I_s(t)) > 0$ .**

ii.  $s.\text{reset}_t(t) = \text{false}$ :

By property of  $\gamma, E_c, \tau \vdash s \overset{\uparrow}{\sim} \sigma$  and  $s.\text{reset}_t(t) = \text{false}$ :

$$\sigma(id_t)("src") = \text{false} \quad (1.52)$$

Case analysis on  $s.I(t) > \text{upper}(I_s(t))$  or  $s.I(t) \leq \text{upper}(I_s(t))$ :

$$\text{A. } s.I(t) > \text{upper}(I_s(t)): \boxed{\sigma'(id_t)("stc") = \text{upper}(I_s(t))}.$$

By definition of  $E_c, \tau \vdash s \overset{\downarrow}{\rightarrow} s'$ :

$$s'.I(t) = s.I(t) \quad (1.53)$$



By definition of  $\gamma, E_c, \tau \vdash s \overset{\uparrow}{\sim} \sigma$ :

$$\sigma(id_t)("stc") = upper(I_s(t)) \quad (1.54)$$

Thanks to (1.25):

$$\sigma'(id_t)("stc") = \sigma(id_t)("stc") \quad (1.55)$$

Rewriting the goal with (1.55) and (1.54): **tautology.**

$$\text{B. } s.I(t) = lower(I_s(t)): \boxed{\sigma'(id_t)("stc") = lower(I_s(t))}.$$

By definition of  $\gamma, E_c, \tau \vdash s \overset{\uparrow}{\sim} \sigma$ :

$$s.I(t) = \sigma(id_t)("stc") \quad (1.56)$$

Thanks to (1.25):

$$\sigma'(id_t)("stc") = \sigma(id_t)("stc") \quad (1.57)$$

Rewriting the goal with (1.57), (1.56) and  $s.I(t) = lower(I_s(t))$ : **tautology.**

$$4. \boxed{upper(I_s(t)) \neq \infty \wedge s'.I(t) \leq upper(I_s(t)) \Rightarrow s'.I(t) = \sigma'(id_t)("s\_time\_counter")}.$$

□

### 1.6.3 Falling edge and firable transitions

**Lemma 9** (Falling Edge Equal Firable). *For all  $sitpn, d, \gamma, \Delta, \sigma_e, E_c, E_p, \tau, s, s', \sigma, \sigma_i, \sigma_{\downarrow}, \sigma'$  that verify the hypotheses of Def. 1, and  $\forall t, id_t$  s.t.  $\gamma(t) = id_t$  and  $\sigma'(id_t) = \sigma'_t$ , then  $t \in Firable(s') \Leftrightarrow \sigma'_t("s\_firable") = \text{true}$ .*

*Proof.*

□

## 1.7 A detailed proof: equivalence of fired transitions



## Appendix A

# Reminder on natural semantics



## Appendix B

# Reminder on induction principles

- Present all the material that will be used in the proof, and that needs clarifying for people who do not come from the field (e.g, automaticians and electronicians)
  - structural induction
  - induction on relations
  - ...